S. 39 Nr. 8

$f_a(x)=x^2-ax^3+1$ $(a\neq0)$

$f'_a(x)=2x-3ax^2$

$f''_a(x)=2-6ax$

$f'''_a(x)=-6a$

a)

$f_a(x)$ hat einen Wendepunkt, wenn es ein $x$ gibt, sodass $f''_a(x)=0$ und $f'''_a(x)\neq0$


$\begin{aligned}
&f''_a(x)=0\\
\implies&2-6ax=0\\
\iff&3ax=1\\
\iff&x=\dfrac{1}{3a}\\
\end{aligned}$

$\begin{aligned}
&f'''_a\left(\dfrac{1}{3a}\right)=-6a
\end{aligned}$

Weil $a\neq0$ ist $-6a\neq0$.


b)

$x=\dfrac{1}{3a}$

$y=f\left(\dfrac{1}{3a}\right)
=\dfrac{1}{9a^2}-\dfrac{a}{27a^3}+1\\
=\dfrac{3}{27a^2}-\dfrac{1}{27a^2}+1\\
=\dfrac{2}{27a^2}+1\\
=\dfrac23\cdot\left(\dfrac1{3a}\right)^2+1\\
=\dfrac23x^2+1$

