S. 89 Nr. 26

$$f_r(x)=\sqrt{r^2-x^2}$$

a)

$$f_3(x)=\sqrt{9-x^2}$$

$$f^2_3(x)=9-x^2$$

$$F^2_3(x)=9x-\frac13x^3$$

$$\begin{aligned}
V=&\pi\cdot\int_{-3}^3f^2_3(x)\,dx\\
=&\pi\cdot\left[F^2_3(x)\right]_{-3}^3\\
=&\pi\cdot(18-(-18))\\
=&36\pi
\end{aligned}$$

$$\begin{aligned}
V=&\frac43\pi r^3\\
=&36\pi
\end{aligned}$$

b)

$$f^2_r(x)=r^2-x^2$$

$$F^2_r(x)=r^2x-\frac13x^3$$

$$\begin{aligned}
V=&\pi\cdot\int_{-r}^rf^2_r(x)\,dx\\
=&\pi\cdot\left[F^2_r(x)\right]_{-r}^r\\
=&\pi\cdot\left(\frac23r^3-\left(-\frac23r^3\right)\right)\\
=&\pi\cdot\frac43\cdot r^3\\
=&\frac43\pi r^3
\end{aligned}$$

HA: S. 89 Nr. 27