S. 40 Nr 14

c)

$f_k(t)=0.5t^3-1.5kt^2+6kt-6t+50$

$\begin{aligned}
&f_{k_1}(t)=f_{k_2}(t)\\
\implies&0.5t^3-1.5k_1t^2+6k_1t-6t+50=0.5t3-1.5k_2t^2+6k_2t-6t+50\\
\iff&-1.5k_1t^2+6k_1t=-1.5k_2t^2+6k_2t\\
\iff&-1.5k_1t^2+6k_1t+1.5k_2t^2-6k_2t=0\\
\implies&t=0\quad\lor\quad1.5k_1t+6k_1+1.5k_2t-6k_2=0
\end{aligned}$

$\begin{aligned}
&-1.5k_1t+6k_1+1.5k_2t-6k_2=0\\
\iff&-1.5k_1t+1.5k_2t=6k_2-6k_1\\
\iff&1.5t\cdot(k_2-k_1)=6k_2-6k_1\\
\iff&t\cdot(k_2-k_1)=4\cdot(k_2-k_1)\\
\iff&t=4
\end{aligned}$

a)

$f_k(t)=0.5t^3-1.5kt^2+6kt-6t+50$

$f'_k(t)=1.5t^2-3kt+6k-6$

$f''_k(t)=3t-3k$

$\begin{aligned}
&f'_k(t)=0
\implies&1.5t^2-3kt+6k-6=0\\
\iff&t^2-2t+4k-4=0\\
\iff&
\end{aligned}$