S. 139 Nr. 2 e) f) g)

e)

$f(x)=\ln(2x-4)$

$f'(x)=(2x-4)^{-1}\cdot2$

f)

$f(x)=ln(x^2)$

$f'(x)=x^{-2}\cdot 2x$

g)

$f(x)=3x\cdot\ln(2x)$

$f'(x)=3\cdot\ln(2x)+3x\cdot(2x)^{-1}\cdot2$


$
u(x)=3x\\
v(x)=ln(x)\\
w(x)=2x\\
$

$g = v \circ w$

$g(x)=v(w(x))=\ln(2x)$

$g'(x)=(2x)^{-1}\cdot2$

Produktregel für $u, v \circ w$

Kettenregel für $v, w$

---

S. 145 Nr. 4 d) e)

d)

$f(x)=e^{2x^2-5}$

$f(-x)=e^{2(-x)^2-5}=e^{2x^2-5}=f(x)$

Achsensymetrisch

e)

$f(x)=x\cdot(e^x+e^{-x})$

$f(-x)=-x\cdot(e^{-x}+e^x)=-f(x)$

Punktsymetrisch

---

