Kettenregel:

$$(u\circ v)'(x_{0})=u'(v(x))\cdot v'(x)$$

---

$f(x)=\sqrt{3x^2-x}$

$f'(x)=\frac12(3x^2-x)^{-\frac12}\cdot(6x-1)$

---

$f(x)=sin(x^3)$

$f'(x)=cos(x^3)\cdot3x^2$'

---

$f(x)=e^{x^4}$

$f'(x)=e^{x^4}\cdot(4x^3)$

---

S. 139 Nr. 1 b) d) f) h) o) p), 2 a)-d)

1

b)

$f(x)=\left(\frac12-5x\right)^3$

$f'(x)=3\cdot\left(\frac12-5x\right)^2\cdot (-5)$

d)

$f(x)=\frac14(x^2-5)^2$

$f'(x)=\frac18(x^2-5)\cdot2x$

f)

$f(x)=e^{-4x}$

$f'(x)=e^{-4x}\cdot(-4)$

h)

$f(x)=e^{-3x-2}$

$f'(x)=e^{-3x-2}\cdot(-3)$

o)

$f(x)=(x+1)\cdot e^{3x}$

$f'(x)=e^{3x}+(x+1)\cdot 3e^{3x}$

p)

$f(x)=(x^2+3x)\cdot e^{2x}$

$f'(x)=(2x+3)\cdot e^{2x}+(x^2+3x)\cdot 2e^{2x}$

2

a)

$f(x)=2e^{x^3-x^2}$

$f'(x)=2e^{x^3-x^2}\cdot (3x^2-2x)$

b)

$f(x)=e^{\sqrt{x}}$

$f'(x)=e^{\sqrt{x}}\cdot\frac12x^{-\frac12}$

c)

$f(x)=e^{\sin(x)+x}$

$f'(x)=e^{\sin(x)+x}\cdot(\cos(x)+1)$

d)

$f(x)=xe^{x^2+2}$

$f'(x)=1\cdot(e^{x^2+2})+x\cdot(e^{x^2+2}\cdot(2x))$
