$$
A(2|-3|0)\\
B(2|2|0)\\
C(-1|2|0)\\
D(-1|-3|0)\\
E(2|-3|5)\\
F(2|2|5)\\
G(-1|2|5)\\
H(-1|-3|5)\\
$$

b)

$$\begin{aligned}
&|\overrightarrow{AG}|\\
=&\sqrt{(2-(-1))^2+(-3-2)^2+(0-5)^2}\\
=&\sqrt{3^2+5^2+5^2}\\
=&\sqrt{59}\\
\approx&7.6811457478686
\end{aligned}$$

S. 177 Nr. 2 e), 4, 5 a), 7 a)

2 e)

$$\begin{aligned}|\overrightarrow{AB}|&=\sqrt{(2-0)^2+(2-(-1))^2+(-2-5)^2}\\
&=\sqrt{2^2+3^2+7^2}\\
&=\sqrt{4+9+49}\\
&=\sqrt{62}\\
&\approx7.874008
\end{aligned}$$

4

$$\begin{aligned}
&3=\sqrt{(5-4)^2+(0-(-2))^2+(p_3-5)^2}\\
\iff&3=\sqrt{5+(p_3-5)^2}\\
\implies&9=5+(p_3-5)^2\\
\iff&4=(p_3-5)^2\\
\iff&p_3-5=2\lor p_3-5=-2\\
\iff&p_3=7\lor p_3=3
\end{aligned}$$

5 a)

$$\begin{pmatrix}5\\7\\6\\\end{pmatrix}$$

7 a)

$$\overrightarrow{AB}=\begin{pmatrix}
3-2\\3-1\\7-4\\
\end{pmatrix}=\begin{pmatrix}
1\\2\\3\\
\end{pmatrix}$$

$$\overrightarrow{d}+\overrightarrow{AB}=\begin{pmatrix}
1+1\\2+3\\3+5\\
\end{pmatrix}=\begin{pmatrix}
2\\5\\8\\
\end{pmatrix}=
\overrightarrow{c}$$

8 a)

$$\overrightarrow{BA}=\begin{pmatrix}
3-2\\1-0\\2-(-2)\\
\end{pmatrix}=\begin{pmatrix}
1\\1\\4\\
\end{pmatrix}$$

$$\overrightarrow{c}+\overrightarrow{BA}=\begin{pmatrix}
1+1\\1+1\\1+4\\
\end{pmatrix}=\begin{pmatrix}
2\\2\\5\\
\end{pmatrix}=\overrightarrow{d}$$

9 a)

$$\overrightarrow{AB}=\begin{pmatrix}
5-2\\2-1\\3-1\\
\end{pmatrix}=\begin{pmatrix}
3\\1\\2\\
\end{pmatrix}$$

$$\overrightarrow{CB}=\begin{pmatrix}
5-3\\2-0\\3-0\\
\end{pmatrix}=\begin{pmatrix}
2\\2\\3\\
\end{pmatrix}$$

$$\overrightarrow{AC}=\begin{pmatrix}
3-2\\0-1\\0-1\\
\end{pmatrix}=\begin{pmatrix}
1\\-1\\-1\\
\end{pmatrix}$$

$$\overrightarrow{AB}\cdot\overrightarrow{AC}=3-1-2=0$$

$$AB\perp AC$$

$$\begin{aligned}
\frac12\cdot|\overrightarrow{AB}|\cdot|\overrightarrow{AC}|&=\frac12\cdot\sqrt{3^2+1^2+2^2}\cdot\sqrt{1^2+(-1)^2+(-1)^2}\\
&=\frac12\cdot\sqrt{9+1+4}\cdot\sqrt{3}\\
&=\frac12\cdot\sqrt{14}\cdot\sqrt{3}\\
&=3.23\quad\text{(FE)}
\end{aligned}$$