Vollstaendige Induktion Ueben

a)

Zu beweisen: $$\forall n\in\mathbb{N}\sum_{i=0}^n(i)=\frac{n^2+n-2}{2}$$

IS:

ISV: $$\sum_{i=0}^n(i)=\frac{n^2+n-2}{2}$$

ZZ: $$\forall n\in\mathbb{N}\quad\text{ISV}\implies\sum_{i=0}^{n+1}(i)=\frac{(n+1)^2+(n+1)-2}{2}$$

ISF: $$\begin{aligned}
&\sum_{i=0}^{n+1}(i)\\
=&\sum_{i=0}^n(i)+(n+1)\\
\overset{ISV}{=}&\frac{n^2+n-2}{2}+(n+1)\\
=&\frac{n^2+n-2+2n+2}{2}\\
=&\frac{n^2+2n+1+n-1}{2}\\
=&\frac{(n+1)^2+(n+1)-2}{2}\\
\end{aligned}$$

IA:

ZZ: $$\sum_{i=0}^1(i)=\frac{1^2+1-2}{2}$$


$$\sum_{i=0}^1(i)=1\neq0=\frac{1^2+1-2}{2}$$

---

b)

Zu Beweisen:

$$\forall n \in\mathbb{N}\sum_{k=1}^{2n}((-1)^k\cdot k)=n$$

IS:

ISV:

$$\sum_{k=1}^{2n}((-1)^k\cdot k)=n$$

ZZ: $$\forall n\in\mathbb{N}\quad\text{ISV}\implies\sum_{k=1}^{2n+2}((-1)^k\cdot k)=n+1$$

ISF: $$\begin{aligned}
&\sum_{k=1}^{2n+2}((-1)^k\cdot k)\\
=&\sum_{k=1}^{2n}((-1)^k\cdot k)+((-1)^{2n+1}\cdot (2n+1))+((-1)^{2n+2}\cdot (2n+2))\\
\overset{\text{ISV}}{=}&n-2n-1+2n+2\\
=&n+1
\end{aligned}$$

IA:

ZZ: $$\sum_{k=1}^{2}((-1)^k\cdot k)=1$$

$$\sum_{k=1}^{2}((-1)^k\cdot k)=-1+2=1$$

c)

Zu Beweisen:

$$\forall n\in\mathbb{N}\sum_{k=0}^n(x^k)=\frac{x^{n+1}-1}{x-1}$$

IS:

ISV: $$\sum_{k=0}^n(x^k)=\frac{x^{n+1}-1}{x-1}$$

ZZ: $$\forall n\in\mathbb{N}\quad\text{ISV}\implies\sum_{k=0}^{n+1}(x^k)=\frac{x^{(n+1)+1}-1}{x-1}$$

ISF:

$$\begin{aligned}
&\sum_{k=0}^{n+1}(x^k)\\
=&\sum_{k=0}^n(x^k)+x^{n+1}\\
\overset{\text{ISV}}=&\frac{x^{n+1}-1}{x-1}+x^{n+1}&\\
=&\frac{x^{n+1}-1}{x-1}+\frac{(x-1)\cdot x^{n+1}}{x-1}\\
=&\frac{x^{n+1}-1}{x-1}+\frac{x\cdot x^{n+1}-x^{n+1}}{x-1}\\
=&\frac{x^{n+1}-1}{x-1}+\frac{x^{(n+1)+1}-x^{n+1}}{x-1}\\
=&\frac{x^{(n+1)+1}-1}{x-1}
\end{aligned}$$

IA:

ZZ: $$\sum_{k=0}^0(x^k)=\frac{x^{0+1}-1}{x-1}$$

$$\sum_{k=0}^0(x^k)=x^0=1=\frac{x-1}{x-1}=\frac{x^{0+1}-1}{x-1}$$

$\Box$


---

AB: Ein letztes AB zur vollstaendigen Induktion

a)

$$a^2+b^2\neq a^2+2ab+b^2=(a+b)^n$$

b)

$$$$