S. 398 Nr. 12

a)

$$E: \vec{x}=\vec{a}+s(\vec{b}-\vec{a})+t(\vec{c}-\vec{a})$$

oder

$$E: (\vec{x}-\vec{a})\cdot((\vec{b}-\vec{a})\times(\vec{c}-\vec{a}))=0$$

Einsetzen von $\vec{x}=\vec{d}$

$$\begin{pmatrix}1\\-6\\2\end{pmatrix}\cdot\left(\begin{pmatrix}3\\1\\2\end{pmatrix}\times\begin{pmatrix}1\\1\\1\end{pmatrix}\right)=\begin{pmatrix}1\\-6\\2\end{pmatrix}\cdot\begin{pmatrix}-1\\-1\\2\end{pmatrix}=9$$

$$9\neq0$$

$D$ liegt nicht auf $E$

b)

$$g: \vec{x}=\vec{d}+s\cdot\begin{pmatrix}24\\-2\\11\end{pmatrix}$$

$$\begin{pmatrix}24\\-2\\11\end{pmatrix}\cdot((\vec{b}-\vec{a})\times(\vec{c}-\vec{a}))=-24+2+22=0$$

$$(\vec{d}-\vec{a})\cdot((\vec{b}-\vec{a})\times(\vec{c}-\vec{a}))\cdot\frac{1}{\left|((\vec{b}-\vec{a})\times(\vec{c}-\vec{a}))\right|}=\begin{pmatrix}1\\-6\\2\end{pmatrix}\cdot\begin{pmatrix}-1\\-1\\2\end{pmatrix}\cdot\frac{1}{\sqrt{(-1)^2+(-1)^2+2^2}}=\frac{9}{\sqrt{6}}\approx3.6742346$$

c)

$$\vec{n}=(\vec{b}-\vec{a})\times(\vec{c}-\vec{a})=\begin{pmatrix}-1\\-1\\2\end{pmatrix}$$

$$\vec{d}-\frac{\vec{n}}{|\vec{n}|}\cdot\frac{9}{\sqrt{6}}=\vec{d}-\begin{pmatrix}-1.5\\-1.5\\3\end{pmatrix}=\begin{pmatrix}3.5\\1.5\\-1\end{pmatrix}$$

$$h: \vec{x}=\begin{pmatrix}3.5\\1.5\\-1\end{pmatrix}+s\cdot\begin{pmatrix}24\\-2\\11\end{pmatrix}$$

d)

$$|CF|=\frac{(\vec{b}-\vec{a})\times(\vec{c}-\vec{a})}{|\vec{b}-\vec{a}|}\approx2.924333109946785$$

$$A_{\triangle ABC}=\frac{1}{2}\cdot|\vec{b}-\vec{a}|\cdot|CF|\approx7.874$$
