$$f(x)=6^x$$

$$\begin{aligned}
f'(x)&=f'(0)\cdot6^x\\
&=\lim_{h\to0}\frac{6^{0+h}-6^0}{h}\\
\end{aligned}$$

S. 105 Nr. 1 a) d) e) g)

a)
$$f(x)=e^x+1$$
$$f'(x)=e^x$$
$$f''(x)=e^x$$

d)
$$f(x)-e^x+1$$
$$f'(x)=-e^x$$
$$f''(x)=-e^x$$

e)
$$f(x)=2e^x+3x^2$$
$$f'(x)=2e^x+6x$$
$$f''(x)=2e^x+6$$

g)
$$f(x)=-\frac12(e^x-x^3)$$
$$f'(x)=-\frac12e^x+\frac32x^2$$
$$f''(x)=-\frac12e^x+3x$$

Nr. 3

a)

$$\begin{aligned}
&\int_{0}^{1}(e^x-x)\,dx\\
=&\int_0^1e^x\,dx-\int_0^1x\,dx\\
=&\left[e^x\right]_0^1-\left[\frac12x^2\right]_0^1\\
=&e^1-e^0-\left(\frac12\cdot1^2-\frac12\cdot0^2\right)\\
=&e-1-\frac12\\
=&e-1\frac12\\
\end{aligned}$$

c)

$$\begin{aligned}
&\int_{-1}^1\left(x^2+\frac15e^x\right)\,dx\\
=&\left[\frac13x^3+\frac15e^x\right]_{-1}^1\\
=&\frac13+\frac15e+\frac13-\frac15e^{-1}\\
=&\frac23+\frac15e-\frac15e^{-1}
\end{aligned}$$


---

S. 109 Nr. 1 a)c)d)f)e)

a)
$$\begin{aligned}
&e^x=15\\
\iff&x=\ln(15)
\end{aligned}$$

c)
$$\begin{aligned}
&e^{2x}=7\\
\iff&2x=\ln(7)\\
\iff&x=\frac{\ln(7)}2\\
\end{aligned}$$

d)
$$\begin{aligned}
&3\cdot e^{4x}=16.2\\
\iff&e^4x=\frac{16.2}3\\
\iff&4x=\ln\left(\frac{16.2}3\right)\\
\iff&x=\frac{\ln\left(\frac{16.2}3\right)}{4}
\end{aligned}$$

f)
$$\begin{aligned}
&e^{4-x}=1\\
\iff&4-x=0\\
\iff&x=4
\end{aligned}$$

l)
$$\begin{aligned}
&-\frac76\cdot e^{-\frac23x+0.5}=\frac67\\
\iff&e^{-\frac23x+0.5}=-\frac{36}{49}\\
\iff&-\frac23x+0.5=\ln\left(\frac{36}{49}\right)\\
\iff&-\frac23x=\ln\left(\frac{36}{49}\right)-0.5\\
\iff&x=-\frac{3\cdot\left(\ln\left(\frac{36}{49}-0.5`\right)\right)}{2}
\end{aligned}$$