19 a) - c)

Dokumentation in der Klausur:

a)

$$\int_{-1}^0(-x^4+5)\,dx=\left[-\frac15x^5+5x\right]_{-1}^0\approx4.8$$

---

Rechenregeln fuer Integrale:

$$\int_a^bf(x)\,dx=-\int_b^af(x)\,dx$$

$$\int_a^bf(x)dx+\int_b^cf(x)\,dx=\int_a^cf(x)\,dx$$

$$\int_a^bc\cdot f(x)\,dx=c\cdot\int_a^bf(x)\,dx$$

$$\int_a^b\left(f(x)+g(x)\right)dx=\int_a^bf(x)\,dx+\int_a^bg(x)\,dx$$

---

S. 68 Nr. 11

a)

$$\begin{aligned}
&\int_{-1}^{3.3}5x^2\,dx-10\int_{-1}^{3.3}\frac12x^2\,dx\\
=&\int_{-1}^{3.3}5x^2\,dx-\int_{-1}^{3.3}5x^2\,dx\\
=&0
\end{aligned}
$$

b)

$$\begin{aligned}
&\int_0^1(x-2\sqrt{x^2-4})\,dx+2\int_0^1\sqrt{x^2+4}\,dx\\
=&\int_0^1x\,dx\\
=&.5
\end{aligned}$$

c)
$$\begin{aligned}
&\int_{-2}^1(2x)\,dx+\int_1^3(2x)\,dx\\
=&\int_{-2}^3(2x)\,dx\\
=&5
\end{aligned}$$

---

S. 67 Nr 2 a b f g

a)
$$F(x)=-\frac14x^{-1}$$

b)
$$F(x)=-x^{-3}$$

f)
$$F(x)=-\frac1{30}x^{-9}$$

g)
$$F(x)=\frac13x^3+\frac12x^2-\frac13x^{-3}$$

---

S. 67 Nr 4d)
$$\begin{aligned}
&\int_0^9\frac25\sqrt{x}\,dx\\
=&\frac25\cdot\int_0^9x^{\frac12}\,dx\\
=&\frac25\cdot\left[\frac23x^{\frac32}\right]_0^9\\
=&\frac25\cdot(0-\frac23\cdot27)\\
=&\frac25\cdot(0-18)\\
=&\frac25\cdot-18\\
=&\frac{36}5
\end{aligned}$$

---

3a)

$$f(x)=0.5x^2-3x=\frac12\cdot x\cdot(x-6)$$

$$\begin{aligned}
&f(x)=0\\
\iff&x=0\lor x=6
\end{aligned}$$

$$\int_0^6f(x)\,dx\\
=\left[\frac16x^3-\frac32x^2\right]_0^6\\
=0-36+54=18$$

---

HA: S. 72 3c+e

c)

$$f(x)=x^4-4x^2$$

$$\begin{aligned}
&f(x)=0\\
\iff&x^4-4x^2=0\\
\iff&x=0 \lor x^2-4=0\\
\iff&x=0 \lor x=2 \lor x=-2\\
\end{aligned}$$

$$F(x)=\frac15x^5-\frac43x^3$$

$$\begin{aligned}
&\left|\int_{-2}^0f(x)\,dx\right|+\left|\int_0^2f(x)\,dx\right|\\
=&\left|\left[F(x)\right]\right|_{-2}^0+\left|\left[F(x)\right]_0^2\right|\\
=&\left|F(0)-F(-2)\right|+\left|F(2)-F(0)\right|\\
=&\left|0-\frac{64}{15}\right|+\left|-\frac{64}{15}-0\right|\\
=&\frac{128}{15}\quad(FE)
\end{aligned}$$

e)

$$f(x)=2x^3-6x^2+4x$$

$$\begin{aligned}
&f(x)=0\\
\iff&2x^3-6x^2+4x=0\\
\iff&x=0 \lor 2x^2-6x+4=0\\
\iff&x=0 \lor x^2-3x+2=0\\
\iff&x=0 \lor (x-1)\cdot(x-2)=0\\
\iff&x=0 \lor x=1 \lor x=2
\end{aligned}$$

$$F(x)=\frac12x^4-2x^3+2x^2$$

$$\vdots$$