Zusammengesetzte Funktionen


$$
\begin{aligned}
f'(x)&=\lim_{h\to 0}\frac {f(x+h)-f(x)}{h}\\
&=\lim_{h\to 0}\frac {u(x+h)\cdot v(x+h)-u(x)\cdot v(x)}{h}\\
&=\lim_{h\to 0}\frac {u(x+h)\cdot v(x+h)-u(x)\cdot v(x+h)+u(x)\cdot v(x+h)-u(x)\cdot v(x)}{h}\\
&=\lim_{h\to 0}\frac {(u(x+h)-u(x))\cdot v(x+h)+u(x)\cdot (v(x+h)-v(x))}{h}\\
&=\lim_{h\to 0}\left(\frac{u(x+h)-u(x)}{h}\cdot v(x+h)+u(x)\cdot {\frac {v(x+h)-v(x)}{h}}\right)\\
&=u'(x)\cdot v(x)+u(x)\cdot v'(x).
\end{aligned}
$$

S. 136 Nr. 1 a) d) i) k)

a)

$$f(x)=2x\cdot(4x-1)=8x^2-2x$$

$$f'(x)=16x-2$$

d)

$$f(x)=2x\cdot e^x$$

$$f'(x)=2\cdot e^x + 2x\cdot e^x$$

i)

$$f(x)=(x^2+x-1)\cdot e^x$$

$$f'(x)=(2x+1)\cdot e^x + (x^2+x-1)\cdot e^x$$

k)

$$f(x)=(x^2-x)\cdot e^{-x}$$

$$f'(x)=(2x-1)\cdot e^{-x}+(x^2-x)\cdot -e^{-x}$$

Nr. 2 b) d)

b)

$$f(x)=\frac1x\cdot e^{2x}$$

$$f'(x)=-x^{-2}\cdot e^{2x}+x^{-1}\cdot 2e^{2x}$$

d)

$$f(x)=\sqrt{x}\cdot e^x=x^{\frac12}\cdot e^x$$

$$f'(x)=\frac12x^{-\frac12}\cdot e^x + x^{\frac12}\cdot e^x$$

Nr. 3 c) 

$$f(x)=(4x-1)\cdot e^x$$

$$f'(x)=4\cdot e^x+ (4x-1)\cdot e^x=(4x+3)\cdot e^x$$

$$f''(x)=4e^x+(4x+3)e^x=(4x+7)e^x$$

$$\begin{aligned}
&f'(x)=0\\
\iff&(4x+3)\cdot e^x=0\\
\iff&e^x=0\lor 4x+3=0\\
\iff&4x+3=0\\
\iff&x=-\frac34
\end{aligned}$$

$$f''\left(-\frac34\right)\approx 1.88946621\neq0$$



HA: Nr. 5

a)

