S. 169 Nr. 14

---

a)

$$f_t(x)=tx\cdot e^{-x^2}$$

$$f_t(0)=0$$

$$\begin{aligned}
&f_t(x)=0\\
\iff&tx\cdot e^{-x^2}=0\\
\iff&tx=0\lor e^{-x^2}=0\\
\iff&x=0
\end{aligned}$$

Der Graph schneidet die Achsen bei $(0,0)$.

$$f_t(x)=tx\cdot e^{-x^2}=t\cdot e^{\ln(x)}\cdot e^{-x^2}=t\cdot e^{-x^2+\ln(x)}$$

$$ln(x)-x^2<0$$

$$\lim_{x\to\infty}f_t(x)=0$$

Und weil $f(-x)=-f(x)$:

$$\lim_{x\to\infty}f_t(x)=0$$

---

b)

$$f_t(-x)=-tx\cdot e^{-x^2}=-f_t(x)$$

Achsensymetrie, aber keine Spiegelsymetrie.

---

c)

$$F_t(x)=-\frac{t}{2}\cdot e^{-x^2}$$

$$\begin{aligned}
F_t'(x)=&\left(-\frac{t}{2}\right)'\cdot e^{-x^2}-\frac{t}{2}\cdot\left(e^{-x^2}\right)'\\
=&0-\frac{t}{2}\cdot(e^{-x^2}\cdot(-2x))\\
=&0+tx\cdot e^{-x^2}\\
=&f_t(x)
\end{aligned}$$

---

d)

$$\int_0^a f_t(x)\,dx=F_t(a)-F_t(0)=F_t(a)-\left(-\frac{t}{2}\right)$$

---

e)

$$\lim_{a\to\infty}F_t(a)=0$$

$$\lim_{a\to\infty}\int_0^af_t(x)\,dx=\lim_{a\to\infty}F_t(a)-\left(-\frac{t}{2}\right)=\frac{t}{2}$$

3